week7 result
status
- stackWasm (was named miniWasm)
  - structure 90+%
  - validation (relational) 90+%
  - execution 90+%

- refactoring
  - moved to multi-value proposal
  - CoqMakefile works
  - rename constructors to UpperCamelCase (naming convention gradualy established)
  - dependency ordering can't follow the spec
    - Int/Float (<- Types) <- Value <- ...
    - influenced from ocaml ref interpreter

- (solved) challenges
  - Numerics / Int / Float / Value modules
    - heavily borrowed from ocaml ref interpreter
  - choose to be more faithfully (eyeball-closeness)
    - evaluation context
    - blocking context
    - frame switching

todo
- meta-theory proof
  - progress
  - preservation
  - soundness

coq/Execution.v
@@ -10,8 +10,7 @@
 (** * Execution *)
 
 From Wasm Require Export Structure.
-
-
+From Wasm Require Export Numerics.
 
 (* ================================================================= *)
 (** ** Runtime Structure *)
@@ -21,11 +20,7 @@ From Wasm Require Export Structure.
 (* ----------------------------------------------------------------- *)
 (** *** Values *)
 
-Inductive val :=
-  | const_i32 : i32 -> val
-  | const_i64 : i64 -> val
-  | const_f32 : f32 -> val
-  | const_f64 : f64 -> val.
+(** Defined in [Values.v] *)
 
 
 (* ----------------------------------------------------------------- *)
@@ -34,8 +29,8 @@ Inductive val :=
 (** In the current version of WebAssembly, a result can consist of at most one value. *)
 
 Inductive result :=
-  | R_val: list val -> result
-  | R_trap.
+  | R_val (_: list val)
+  | R_trap. (* coincident with [trap] *)
 
 
 (* ----------------------------------------------------------------- *)
@@ -53,26 +48,122 @@ Notation globaladdr := addr.
 
 Record moduleinst :=
   {
-    types : list functype;
-    funcaddrs : list funcaddr;
-    (* tableaddrs : list tableaddr; *)
+    MI_types : list functype;
+    MI_funcaddrs : list funcaddr;
+    MI_tableaddrs : list tableaddr;
     (* memaddrs : list memaddr; *)
     (* globaladdrs : list globaladdr; *)
     (* exports : list exportinst; *)
   }.
 
+Definition empty_moduleinst :=
+  {|
+    MI_types := [];
+    MI_funcaddrs := [];
+    MI_tableaddrs := [];
+  |}.
+
 
 (* ----------------------------------------------------------------- *)
 (** *** Function Instances *)
 
-(** hostfunc case is ignore for now *)
+Print Structure.func.
 
-Record funcinst :=
+(* [func] is the AST func: 
+     - type signature [F_type   : typeidx]
+     - locals type    [F_locals : list valtype]
+     - actual code    [F_body   : expr]  (expr := list instr)
+
+   [funcinst] is the closure (heap-allocated, as all other "Xinst"):
+     - environment   [FI_module : module_inst]
+     - code pointer  [FI_code   : func]
+     - type          [FI_type   : functype]
+
+   [Frame] is the activation record (on stack): 
+     - return arity  [A_arity  : nat]
+     - actual locals [A_locals : list val]         (taken from stack)   (recorded in frame)
+     - actual mdule  [A_module : moduleinst]       (taken from closure) (recorded in frame)
+     - actual code   [code     : list admin_instr] (lifting from closure)
+ *)
+
+(* 
+   I first modeled func inst as constructor and write own projections
+   since Coq doesn't support ocaml-like inline record
+
+    Inductive funcinst :=
+      | Func (FI_type: functype) (FI_module: moduleinst) (FI_code: func)
+      | Host (FI_type: functype) (FI_hostcode: hostfunc).
+
+   But latern on I realized record + coercions would be more convenient.
+ *)
+
+Inductive hostfunc := .
+
+Record funcinst__wasm :=
   {
-    type : functype;
-    module : moduleinst;
-    code : func;
+    FI_type__wasm : functype;  (* spec overload [type] *)
+    FI_module   : moduleinst;
+    FI_code     : func;
   }.
+
+Record funcinst__host :=
+  {
+    FI_type__host : functype;  (* spec overload [type] *)
+    FI_hostcode : hostfunc;
+  }.
+
+Inductive funcinst :=
+  | FI_wasm (_: funcinst__wasm)
+  | FI_host (_: funcinst__host).
+
+Coercion FI_wasm : funcinst__wasm >-> funcinst.
+Coercion FI_host : funcinst__host >-> funcinst.
+
+(* type is ad-hoc polymorphic *)
+
+Definition FI_type (f: funcinst) : functype :=
+  match f with
+  | FI_wasm f => f.(FI_type__wasm)
+  | FI_host f => f.(FI_type__host)
+  end.
+
+Notation " f '.(FI_type)' " := (FI_type f) (at level 50).
+
+
+(* ----------------------------------------------------------------- *)
+(** *** Table Instances *)
+
+Notation funcelem := (option funcaddr).
+
+Record tableinst :=
+  {
+    TI_elem : list funcelem;
+    TI_max : option I32.t;  (* option u32 *)
+  }.
+
+Definition empty_tableinst :=
+  {|
+    TI_elem := [];
+    TI_max := Some I32.zero;
+  |}.
+
+(* ----------------------------------------------------------------- *)
+(** *** Memory Instances *)
+
+Record meminst :=
+  {
+    MEI_data : list byte;
+    MEI_max : option I32.t;  (* option u32 *)
+  }.
+
+(* ----------------------------------------------------------------- *)
+(** *** Global Instances *)
+
+(* ----------------------------------------------------------------- *)
+(** *** Export Instances *)
+
+(* ----------------------------------------------------------------- *)
+(** *** External Values *)
 
 (* ----------------------------------------------------------------- *)
 (** *** Store *)
@@ -80,50 +171,700 @@ Record funcinst :=
 
 Record store :=
   {
-    funcs : list funcinst;
-    (* tables : list tableinst; *)
-    (* mems : list meminst; *)
-    (* globals : list globalinst; *)
+    S_funcs : list funcinst;
+    S_tables : list tableinst;
+    (* S_mems : list meminst; *)
+    (* S_globals : list globalinst; *)
   }.
+
+Definition empty_store :=
+  {|
+    S_funcs := [];
+    S_tables := [];
+  |}.
 
 
 (* ----------------------------------------------------------------- *)
 (** *** Stack *)
 
-
 (** **** Activations and Frames *)
 
 Record frame :=
   {
-    locals: list val;
-    frame_module: moduleinst;
+    A_locals: list val;
+    A_module: moduleinst;
   }.
 
-Inductive activation :=
-  | Frame (arity : nat) (_ : frame).
+(** activation is coincident with the [Frame] admin_instr *)
+
+Record activation :=
+  {
+    A_arity: nat;
+    A_frame: frame;
+  }.
+
+Definition empty_frame :=
+  {|
+    A_locals := [];
+    A_module := empty_moduleinst;
+  |}.
+
+Definition empty_activation :=
+  {|
+    A_arity := 0;
+    A_frame := empty_frame;
+  |}.
+
+Definition upd_locals (F: frame) (x: nat) (v: val) :=
+  match update_idx F.(A_locals) x v with
+  | None => None
+  | Some vs => Some
+      {|
+        A_locals := vs;
+        A_module := F.(A_module);
+      |}
+  end.
+  
+Notation "F 'with_locals[' x ] = v" :=
+  (upd_locals F x v)
+  (at level 69, left associativity) : wasm_scope.
+
+
+Lemma upd_locals_inv: forall F F' n c,
+  (F with_locals[n] = c) = Some F' ->
+  F'.(A_locals).[n] = Some c.
+Proof.
+  Abort.
+
+
+(* test *)
+
+Module FrameTests.
+
+  Parameter c : val.
+  Parameter c' : val.
+
+  Example F0 := empty_frame.
+  Compute F0.(A_locals).[0].  (* => None *)
+  Compute (F0 with_locals[0] = c). (* => None *)
+
+  Example F1 :=
+    {|
+      A_locals := [c; c];
+      A_module := empty_moduleinst;
+    |}.
+
+  Compute F1.(A_locals).[0].  (* => Some c *)
+  Compute (F1 with_locals[0] = c'). (* => Some F' *)
+
+  Example upd_locals_inv: forall F',
+    (F1 with_locals[0] = c') = Some F' ->
+    F'.(A_locals).[0] = Some c'.
+  Proof with eauto.
+    unfold upd_locals.
+    intros. simpl in *. 
+    inversion H...
+  Qed.
+
+End FrameTests.
+
+
+(** **** Expand *)
+
+(** the original spec doesn't need to take acount of None case.
+    since execution has assumed to pas the validaton
+ *)
+
+Definition expand (F: frame) (bt: blocktype) : option functype :=
+  match bt with
+  | BT_typeidx typeidx => F.(A_module).(MI_types).[typeidx]
+  | BT_valtype opt_valtype => Some ([] --> (opt_to_rt opt_valtype))
+  end.
 
 
 (* ----------------------------------------------------------------- *)
 (** *** Administrative Instructions *)
 
-Inductive instr :=
-  | E_instr (_ : Structure.instr)
-  | E_trap
-  | E_label : nat -> list instr -> list instr -> instr
-  | E_frame : nat -> list frame -> list instr -> instr.
+Inductive admin_instr :=
+  | Plain (_: instr)
+  | Trap
+  | Invoke (closure: funcaddr)
+  | Label (n: nat) (cont: list instr) (code: list admin_instr)
+  | Frame (n: nat) (activation: frame) (code: list admin_instr).
 
 
-(** **** Blocking Contexts *)
+(** lifting *)
+
+Definition lift_plains (is: list instr) : list admin_instr :=
+  List.map (fun i => Plain i) is.
+
+Definition lift_vals(vals: list val) : list instr :=
+  map (fun v => Const v) vals.
+
+(* TBD: need a code to be able to lift to Frame *)
+Definition lift_activation (a: activation) :=
+  Frame a.(A_arity) a.(A_frame).
 
 
-(** **** Configurations *)
+(** Coercions and Notations *)
+(** since the coercion doesn't work well with [list X] so we introduce
+    rather heavy notation for the lifting *)
 
-Notation thread := (frame * (list instr))%type.
+Coercion Plain : instr >-> admin_instr.
 
-Definition config : Type := store * thread.
+Notation "↑ instrs" := (lift_plains instrs) (at level 60).         (* \uparrow *)
+Notation "⇈ vals" := (lift_plains (lift_vals vals)) (at level 50). (* \upuparrows *)
+
+(** test *)
+
+Module AdminInstrCoercisonTest.
+
+  Parameter c : val.
+  Example ain : admin_instr := Nop.
+
+  Fail Example ai__fail : list admin_instr := [Nop].
+
+  Example ais : list admin_instr := ↑[Nop].
+
+  Example avs : list admin_instr := ⇈[c].
+  Example test__app : list admin_instr := ⇈[c] ++ ais.
+
+  Example a : activation :=
+    {|
+      A_arity := 1;
+      A_frame := empty_frame;
+    |}.
+
+End AdminInstrCoercisonTest.
 
 
-(** **** Evaluation Contexts *)
+(* ----------------------------------------------------------------- *)
+(** *** Blocking Contexts *)
+(** https://webassembly.github.io/multi-value/core/exec/runtime.html#block-contexts *)
+
+(** blocking context is coincident with the [Label] admin_instr
+
+    We found some inconsistency about the treatment on this:
+
+    - reference interpreter :
+      * having admin_instr [Breaking] and [Returning] that carried over all the unwinding vals until the [Label n] is reached and it will push the [n] val back.
+      * the "jumping out" from all the blocking contexts is done step-by-step (one-by-one)
+
+    - original paper and Isabelle all use a giganitic step to jump to the target label directly.
+      * the problem is that during the Progress proof of type soundness we will need to build (show the exsistence)
+        all the necessary decomposition of [instrs] anyway.
+
+    - more problematically, in the spec
+      * the formal notation is done in one "gigantic step",
+      * the prose is demonstrated "step-by-step".
+
+    - we will see which one to use
+ *)
+
+
+(* block contexts is defined as a type family indexed by the count of labels surronding a hole,
+   i.e. dependent sum  *)
+
+Inductive block_context : nat -> Type :=
+
+  (* B0 ::= val∗ [_] instr∗  -- this is equiv to E_val *)
+  | B_nil  : forall (vals: list val) (* [_] *) (instrs: list admin_instr),
+               block_context 0
+
+  (* Bk+1 ::= val∗ label n {instr∗} Bk end instr∗  *)
+  | B_cons : forall {k: nat}
+               (vals: list val)
+               (n: nat) (cont: list instr)  (* Label *)
+               (B: block_context k)
+               (instrs: list admin_instr),
+               block_context (k+1).
+
+Fixpoint plug_block_context {k: nat} (B: block_context k) (hole: list admin_instr) : list admin_instr :=
+  match B with
+  | B_nil vals instrs => ⇈ vals ++ hole ++ instrs
+  | B_cons vals n cont B' instrs =>
+      ⇈ vals ++ [Label n cont (plug_block_context B' hole)] ++ instrs
+  end.
+
+Notation plug__B := plug_block_context.
+
+Module BlockContextTest.
+
+  Parameter c : val.
+
+  Example vals := [c; c].
+  Example instrs := ↑[Nop].
+  Example cont := [Nop].
+
+  Example B0 := B_nil vals instrs.
+  Compute (plug__B B0 [Trap]).
+
+  Example B1 := B_cons vals (*label*) 0 cont B0 (*end*) instrs.
+  Compute (plug__B B1 [Trap]).
+
+End BlockContextTest.
+
+
+(* ----------------------------------------------------------------- *)
+(** *** Configurations *)
+
+(** There could be multiple settings on the configurations:
+
+    (1) threading.
+   
+          Notation thread := (frame * (list admin_instr))%type.
+          Notation config := (store * thread)%type.
+
+
+    (2) arbitray [admin_instr\ast] as control, or code
+
+          Notation config := (store * frame * (list admin_instr))%type.
+
+        This has benefit that being closer to the spec sometimes.
+        the spec use the notation of execution context implicitly use
+        the _composed_ version and _decomposed_ version interchangbly.
+
+        The cons are that to do proof on this, we will need to _figure out_
+        the correct decomposition of execution context everytimes...
+        although it should be rather straightforward since we could prove
+        that any [list admin_instr] share the [unique decomposition] properties
+        on the first occurence of [val].
+
+    (3) make code a product type
+
+          Notation code := (list val * list admin_instr)%type.
+          Notation config := (store * frame * code)%type.
+
+        This has the benefit to be closer to the original paper, ref interpeter,
+        and some of the instructions that defined in the decomposed mannar.
+
+        The main reason of doing so is that it made the step relation clear and
+        proof potentially easier beacuse we explicit include this information.
+
+    Potential future Work:
+    One way to enrich our work is to prove the (2) and (3) are equivalent.
+*)
+
+Notation config := (store * frame * list admin_instr)%type.
+
+Definition empty_config : config := (empty_store, empty_frame, []).
+
+
+(* ----------------------------------------------------------------- *)
+(** *** Evaluation Contexts *)
+(** https://webassembly.github.io/multi-value/core/exec/runtime.html#evaluation-contexts *)
+
+(** There are at least 2 types of execution context:
+    It's frank that Frame admin_instr is not a kind of EC.
+
+        E ::= [_]
+            | val⃰ E instr⃰
+            | label_n {instr⃰} E end
+
+    Technically, in the sense of "frame" in contextual semantics:
+
+        Inductive frame : Type :=
+          | F_stack : list val -> list admin_instr -> hole -> frame
+          | F_label : N -> list admin_instr -> hole -> frame
+
+    But they are somewhat overloading and could be coerce: 
+    - val and instr are coincident.
+    - Label EC and Label admin_instr are coincident.
+    - EC has its own configuration... 
+ *)
+
+Inductive eval_context :=
+  | E_hole 
+  | E_seq (vals: list val) (E: eval_context) (instrs: list admin_instr)
+  | E_label (n: nat) (cont: list instr) (E: eval_context).
+
+Fixpoint plug_eval_context (E: eval_context) (hole: list admin_instr) : list admin_instr :=
+  match E with
+   | E_hole => hole
+   | E_seq vals E instrs => ⇈vals ++ (plug_eval_context E hole) ++ instrs
+   | E_label n cont E => [Label n cont (plug_eval_context E hole)]
+  end.
+
+Notation plug__E := plug_eval_context.
+
+
+Module EvalContextTest.
+
+  Parameter c : val.
+
+  Example vals := [c; c].
+  Example instrs := ↑[Nop].
+  Example cont := [Nop].
+
+  Example E0 := E_hole.
+  Example E1 := E_seq vals E0 instrs.
+  Example E2 := E_label 0 cont E1. 
+
+  Compute (plug__E E0 [Trap]).
+  Compute (plug__E E1 [Trap]).
+  Compute (plug__E E2 [Trap]).
+
+End EvalContextTest.
+
+
+
+(* ================================================================= *)
+(** ** Instructions *)
+(** https://webassembly.github.io/multi-value/core/exec/instructions.html#instructions *)
+
+
+(* Failure on [val_of] is a _runtime type error_ (getting stuck).
+   Returning [Trap] is an acceptable result for proving soundness. 
+
+   The reference interepter implicit exploit the property where 
+   there is a 1-1 correspondence between:
+
+        val := @op   I32.t       I64.t    ...
+                      ↓           ↓
+        ops := @op  IOp32.op   IOp64.op   ...
+
+   So we can safely do the [val_of]
+
+
+   here we have two approaches to exploit and prove this:
+
+   (1) We have some predicates making this requirements explicit.
+
+      Inductive rep_of_val {i32 i64 f32 f64 : Type} :
+          forall (ops : @op i32 i64 f32 f64), val -> rep_type_of ops -> Prop :=
+        | RV_i32 : forall i, rep_of_val (i32 _) (i32 i) i
+        | ...
+        .
+
+      Inductive step_simple : list admin_instr -> list admin_instr -> Prop :=
+        | SS_binop__some : forall op c1 v1 c2 v2 c v,
+            rep_of_val op c1 v1 ->
+            rep_of_val op c2 v2 ->
+            eval_binop op v1 v2 = Some v ->
+            rep_of_val op c v ->
+            ↑[Const c1; Const c2; Binop op] ↪s ↑[Const c]
+
+    (2) making these two failures distinct.
+        e.g. here we add a new sum type [runtime_err] besides [option]
+
+        and we then prove [Err] case doesn't exist after validation. 
+ *)
+
+
+(* In terms of name, we might want to merge [SS] and [SC] into one. *)
+
+(* Simple Step *)
+Reserved Notation "instrs1 '↪s' instrs2" (at level 70).
+Inductive step_simple : list admin_instr -> list admin_instr -> Prop :=
+
+(* ----------------------------------------------------------------- *)
+(** *** Numeric Instruction *)
+
+  | SS_unop__some : forall op c1 c,
+      eval_unop op c1 = Ok (Some c) ->
+      ↑[Const c1; Unop op] ↪s ↑[Const c]
+
+  | SS_unop__none : forall op c1,
+      eval_unop op c1 = Ok None ->
+      ↑[Const c1; Unop op] ↪s [Trap]
+
+  | SS_binop__some : forall op c1 c2 c,
+      eval_binop op c1 c2 = Ok (Some c) ->
+      ↑[Const c1; Const c2; Binop op] ↪s ↑[Const c]
+
+  | SS_binop__none : forall op c1 c2, 
+      eval_binop op c1 c2 = Ok None ->
+      ↑[Const c1; Const c2; Binop op] ↪s [Trap]
+
+  | SS_testop: forall op c1 c,
+      eval_testop op c1 = Ok c ->
+      ↑[Const c1; Testop op] ↪s ↑[Const c]
+
+  | SS_relop: forall op c1 c2 c,
+      eval_relop op c1 c2 = Ok c ->
+      ↑[Const c1; Const c2; Relop op] ↪s ↑[Const c]
+
+(* ----------------------------------------------------------------- *)
+(** *** Parametric Instruction *)
+
+  | SS_drop : forall c,
+      ↑[Const c; Drop] ↪s []
+
+  | SS_select1 : forall c1 c2 c,
+      c <> I32.zero ->
+      ↑[Const c1; Const c2; Const (i32 c); Select] ↪s ↑[Const c1]
+
+  | SS_select2 : forall c1 c2 c,
+      c = I32.zero ->
+      ↑[Const c1; Const c2; Const (i32 c); Select] ↪s ↑[Const c2]
+
+(* ----------------------------------------------------------------- *)
+(** *** Control Instruction *)
+
+  | SS_nop : 
+      ↑[Nop] ↪s []
+
+  | SS_unreachable : 
+      ↑[Unreachable] ↪s [Trap]
+
+  | SS_br : forall n instrs l (Bl: block_context l) vals,
+      length vals = n ->
+      [Label n instrs (plug__B Bl (⇈vals ++ ↑[Br l]))] ↪s ⇈vals ++ ↑instrs
+
+  | SS_br_if1 : forall c l,
+      c <> I32.zero ->
+      ↑[Const (i32 c); Br_if l]  ↪s ↑[Br l]
+
+  | SS_br_if2 : forall c l,
+      c = I32.zero ->
+      ↑[Const (i32 c); Br_if l]  ↪s []
+
+  | SS_br_table__i : forall ls l__N l__i (i: nat),
+      ls.[i] = Some l__i ->
+      ↑[Const i; Br_table ls l__N]  ↪s  ↑[Br l__i]
+
+  | SS_br_table__N : forall ls l__N (i: nat),
+      length ls <= i ->
+      ↑[Const i; Br_table ls l__N]  ↪s  ↑[Br l__N]
+
+(* ----------------------------------------------------------------- *)
+(** *** Control Instruction - Function Call Related *)
+
+  | SS_return : forall n F k (Bk : block_context k) vals,
+      length vals = n ->
+      [Frame n F (plug__B Bk (⇈vals ++ ↑[Return]))] ↪s ⇈vals
+
+(* ----------------------------------------------------------------- *)
+(** *** Block *)
+
+  | SS_block__exit : forall n m vals instrs,
+      length vals = m ->
+      [Label n instrs (⇈vals)]  ↪s ⇈vals
+
+(* ----------------------------------------------------------------- *)
+(** *** Function Calls *)
+(** **** Returning from a function *)
+
+  | SS_frame__exit : forall n F vals,
+      length vals = n ->
+      [Frame n F (⇈vals)]  ↪s ⇈vals
+
+where "instrs1 '↪s' instrs2"  := (step_simple instrs1 instrs2).
+
+(* Config Step *)
+Reserved Notation "cfg1 '↪' cfg2" (at level 40).
+Inductive step_config : config -> config -> Prop :=
+
+(* ----------------------------------------------------------------- *)
+(** *** Lifting ↪s *)
+
+  | SC_simple : forall S F instrs instrs',
+      instrs ↪s instrs' ->
+      (S, F, instrs) ↪ (S, F, instrs')
+
+(* ----------------------------------------------------------------- *)
+(** *** Memory Instruction *)
+
+  | SC_local_get : forall S F x v, 
+      F.(A_locals).[x] = Some v ->
+      (S, F, ↑[Local_get x]) ↪ (S, F, ↑[Const v])
+
+  | SC_local_set : forall S F F' x v, 
+      Some F' = F with_locals[x] = v ->
+      (S, F, ↑[Const v; Local_set x]) ↪ (S, F', [])
+
+  | SC_local_tee : forall S F x v, 
+      (S, F, ↑[Const v; Local_tee x]) ↪ (S, F, ↑[Const v; Const v; Local_set x])
+
+  (* | SC_global_get *)
+  (* | SC_global_set *)
+
+(* ----------------------------------------------------------------- *)
+(** *** Control Instruction *)
+
+  (* 这里应该根据 BT 的 n -> m 带 n 个 var 进 Label 里来, 然后标记 label 为 m
+     原 paper 更为正确
+
+     Interpreter 的做法也是正确的....还更新了前面的 val 部分
+
+        let args, vs' = take n1 vs e.at, drop n1 vs e.at in
+        vs', [Label (n2, [], (args, List.map plain es')) @@ e.at]
+
+     In terms of preservation/progress proof, I think we can always extract
+     sufficient number of vals from the well-type premise. 
+   *)
+                                      
+  | SC_block : forall S F m n ts1 ts2 bt instrs vs,
+      m = length ts1 ->
+      n = length ts2 ->
+      length vs = m ->
+      expand F bt = Some (ts1 --> ts2) ->
+      (S, F, vs ++ ↑[Block bt instrs]) ↪ (S, F, [Label n ϵ (vs ++ ↑instrs)])
+
+  | SC_loop : forall S F m n ts1 ts2 bt instrs vs,
+      m = length ts1 ->
+      n = length ts2 ->
+      length vs = m ->
+      expand F bt = Some (ts1 --> ts2) ->
+      (S, F, vs ++ ↑[Loop bt instrs]) ↪ (S, F, [Label n [Loop bt instrs] (vs ++ ↑instrs)])
+
+  (* The original paper definition (and Isabelle) simply desugar [if] into [block]
+     But here we faithfully represent the spec and made the rule explicit. *)
+
+  | SC_if1 : forall S F m n ts1 ts2 bt instrs1 instrs2 c vs,
+      m = length ts1 ->
+      n = length ts2 ->
+      length vs = m ->
+      c <> I32.zero ->
+      expand F bt = Some (ts1 --> ts2) ->
+      (S, F, vs ++ ↑[Const (i32 c); If bt instrs1 instrs2]) ↪ (S, F, [Label n ϵ (vs ++ ↑instrs1)])
+
+  | SC_if2 : forall S F m n ts1 ts2 bt instrs1 instrs2 c vs,
+      m = length ts1 ->
+      n = length ts2 ->
+      length vs = m ->
+      c = I32.zero ->
+      expand F bt = Some (ts1 --> ts2) ->
+      (S, F, vs ++ ↑[Const (i32 c); If bt instrs1 instrs2]) ↪ (S, F, [Label n ϵ (vs ++ ↑instrs2)])
+
+(* ----------------------------------------------------------------- *)
+(** *** Control Instruction - Function Call Related *)
+
+  | SC_call : forall S F x a,
+      F.(A_module).(MI_funcaddrs).[x] = Some a ->
+      (S, F, ↑[Call x]) ↪ (S, F, [Invoke a])
+
+  | SC_call_indirect : forall S F (i: nat) x a (ta: tableaddr) (tab: tableinst) f ft,
+
+      (* S.tables[F.module.tableaddrs[0]].elem[i] = a *)
+
+      F.(A_module).(MI_tableaddrs).[0] = Some ta ->
+      S.(S_tables).[ta] = Some tab ->
+      tab.(TI_elem).[i] = Some (Some a) ->
+
+      S.(S_funcs).[a] = Some f ->
+
+      (* F.module.types[x] = f.type *)
+
+      F.(A_module).(MI_types).[x] = Some ft ->
+
+      (* this [FI_type] is polymorphic over wasm and host *)
+      f.(FI_type) = ft ->
+
+      (* Coercion [nat_to_i32] happened to [i] here. *)
+      (S, F, ↑[Const i; Call_indirect x]) ↪ (S, F, [Invoke a])
+
+  | SS_call_indirect__trap : forall S F i x,
+      (S, F, ↑[Const (i32 i); Call_indirect x]) ↪ (S, F, [Trap])
+
+(* ----------------------------------------------------------------- *)
+(** *** Function Call *)
+
+  | SC_invoke : forall S F' F vals a n m ts1 ts2 instrs f x ts,
+
+      S.(S_funcs).[a] = Some (FI_wasm f) ->
+
+      length ts1 = n ->
+      length ts2 = m ->
+      f.(FI_type) = ts1 --> ts2 ->
+
+      f.(FI_code) = {| F_type := x; F_locals := ts; F_body := instrs |} ->
+
+      F = {| A_module := f.(FI_module); A_locals := vals ++ (zeros ts) |} ->
+
+(*     S;      val^n   (invoke a)  ↪  S;      frame_m{F} label_m {}   instr* end end *)
+      (S, F', ⇈vals ++ [Invoke a]) ↪ (S, F', [Frame m F [Label m [] (↑instrs)]])
+
+(** **** Host Functions *)
+
+  (* | SC_invoke_host  *)
+  (* | SC_invoke_host__trap  *)
+
+(* ----------------------------------------------------------------- *)
+(** *** Evaluation Contexts *)
+
+(*
+       S; F;   instr*  ↪ S′; F′;   instr′*
+    ------------------------------------------
+       S; F; E[instr*] ↪ S′; F′; E[instr′*]
+*)
+
+  | SC_E : forall E S S' F F' instrs instrs',
+      (S, F,         instrs) ↪ (S', F',         instrs') ->
+      (S, F, plug__E E instrs) ↪ (S', F', plug__E E instrs')
+
+(*
+       S;              F'; instr*     ↪ S';             F''; instr′*
+    ----------------------------------------------------------------------
+       S; F;  frame_n {F'} instr* end ↪ S'; F; frame_n {F''} instr'* end
+*)
+
+  | SC_frame : forall S S' F F' F'' n instrs instrs',
+      (S,             F',instrs ) ↪ (S',             F'',instrs' ) ->
+      (S, F, [Frame n F' instrs]) ↪ (S', F, [Frame n F'' instrs'])
+
+(** **** Trap *)
+
+  | SC_trap__E : forall E S F, 
+      (S, F, plug__E E [Trap]) ↪ (S, F, [Trap])
+
+  | SC_trap__frame : forall S F n F', 
+      (S, F, [Frame n F' [Trap]]) ↪ (S, F, [Trap])
+                             
+(* ----------------------------------------------------------------- *)
+(** *** Expressions *)
+(** https://webassembly.github.io/multi-value/core/exec/instructions.html#expressions *)
+(* since
+
+      Definition/Notation expr := list instr
+
+   I am afraid that I have implicitly include this rule all over the place
+   that we define the structure with expr...
+
+   Do we really need this?
+*)
+
+  | SC_expr : forall S S' F F' (e: expr) (e': expr) instrs instrs', 
+    e  = instrs ->
+    e' = instrs' ->
+    (S, F, ↑e) ↪ (S', F', ↑e') ->
+    (S, F, ↑instrs) ↪ (S', F', ↑instrs') 
+
+where "cfg1 '↪' cfg2" := (step_config cfg1 cfg2).
+
+
+
+(* ================================================================= *)
+(** ** Archive (Deprecated) *)
+
+(* Originally, I defined Eval Context as a "pre-filled" things.
+
+      Inductive eval_context :=
+        | E_val (vals: list val) (hole: list admin_instr) (instrs: list admin_instr)
+        | E_label (n: nat) (cont: list instr) (hole: list admin_instr).
+
+   and represent the transition inside a eval context, i.e.
+
+      S; F; E[instr*] ↪ S′; F′; E[instr′*]
+
+   as a step relation on a special version of config via eval context:
+
+      Notation E_config := (store * frame * eval_context)%type.
+
+      Reserved Notation "E_cfg1 '↪' E_cfg2" (at level 40).
+      Inductive step : E_config -> E_config -> Prop :=
+
+        | SC_val : forall S S' F F' vs es instrs instrs',
+            (S, F, instrs) ↪c (S', F', instrs') ->
+            (S, F, (E_val vs instrs es)) ↪ (S', F', (E_val vs instrs' es))
+
+        | SC_label : forall S S' F F' n vs es instrs instrs',
+            (S, F, instrs) ↪c (S', F', instrs') ->
+            (S, F, (E_label n es instrs)) ↪ (S', F', (E_label n es instrs'))
+
+      where "E_cfg1 '↪' E_cfg2" := (step E_cfg1 E_cfg2).
+
+*)
 
 
 
