coq/Validation.v
@@ -10,17 +10,12 @@
 
 From Wasm Require Export Structure.
 From Coq Require Export Structures.Equalities.
-Import FunctypeNotations.
 
 (* Test imports/exports *)
 
 Module ImportExportTests.
 Definition ex_fun_nu : functype := [] --> [T_i32].
-Definition ex_fun_nu_ty_c : ty := [] --> [T_i32].
 Print ex_fun_nu.
-Print ex_fun_nu_ty_c.
-Print ty.
-Print module.
 End ImportExportTests.
 
 
@@ -34,31 +29,50 @@ End ImportExportTests.
 
 Record context :=
   {
-    types : list functype;
-    funcs : list functype;
-    locals : list valtype;
-    labels : list resulttype;
-    return' : option resulttype;
+    C_types : list functype;
+    C_funcs : list functype;
+    C_tables : list tabletype;
+    C_locals : list valtype;
+    C_labels : list resulttype;
+
+    (* this could actually be just a resulttype since [] can represent None *)
+    C_return : option resulttype;  
   }.
 
-
-(** indexing and indexing notation *)
-
-Notation idx := nth_error.
-Notation "l '.[' x ]" :=
-  (idx l x)
-  (at level 60, right associativity) : wasm_scope.
+Definition empty_context :=
+  {|
+    C_types := [];
+    C_funcs := [];
+    C_tables := [];
+    C_locals := [];
+    C_labels := [];
+    C_return := Some [];
+  |}.
 
 
 (** functional update - replacing fields *)
 
+Definition replace_locals(C: context) (xs: list valtype) :=
+  {|
+    C_locals := xs;
+    C_types  := C.(C_types);
+    C_funcs  := C.(C_funcs);
+    C_tables := C.(C_tables);
+    C_labels := C.(C_labels);
+    C_return := C.(C_return);
+  |}.
+Notation "C 'with_locals' = xs" :=
+  (replace_locals C xs)
+  (at level 69, left associativity) : wasm_scope.
+
 Definition replace_labels (C: context) (xs: list resulttype) :=
   {|
-    types := C.(types);
-    funcs := C.(funcs);
-    locals := C.(locals);
-    labels := xs;
-    return' := C.(return');
+    C_labels := xs;
+    C_types := C.(C_types);
+    C_funcs := C.(C_funcs);
+    C_tables := C.(C_tables);
+    C_locals := C.(C_locals);
+    C_return := C.(C_return);
   |}.
 Notation "C 'with_labels' = x" :=
   (replace_labels C x)
@@ -66,11 +80,12 @@ Notation "C 'with_labels' = x" :=
 
 Definition replace_return (C: context) (x: resulttype) :=
   {|
-    types := C.(types);
-    funcs := C.(funcs);
-    locals := C.(locals);
-    labels := C.(labels);
-    return' := Some x;
+    C_return:= Some x;
+    C_types := C.(C_types);
+    C_funcs := C.(C_funcs);
+    C_tables := C.(C_tables);
+    C_locals := C.(C_locals);
+    C_labels := C.(C_labels);
   |}.
 Notation "C 'with_return' = x" :=
   (replace_return C x)
@@ -81,43 +96,32 @@ Notation "C 'with_return' = x" :=
 
 Definition cons_labels (C: context) (x: resulttype) :=
   {|
-    types := C.(types);
-    funcs := C.(funcs);
-    locals := C.(locals);
-    labels := x :: C.(labels);
-    return' := C.(return');
+    C_labels := x :: C.(C_labels);
+    C_types := C.(C_types);
+    C_funcs := C.(C_funcs);
+    C_tables := C.(C_tables);
+    C_locals := C.(C_locals);
+    C_return := C.(C_return);
   |}.
-Notation "C ',' 'labels' x" :=
+Notation "C ',labels' x" :=
   (cons_labels C x)
   (at level 68, left associativity) : wasm_scope.
 
 
 Definition cons_locals (C: context) (x: valtype) :=
   {|
-    types := C.(types);
-    funcs := C.(funcs);
-    locals := x :: C.(locals);
-    labels := C.(labels);
-    return' := C.(return');
+    C_locals := x :: C.(C_locals);
+    C_types := C.(C_types);
+    C_funcs := C.(C_funcs);
+    C_tables := C.(C_tables);
+    C_labels := C.(C_labels);
+    C_return := C.(C_return);
   |}.
-Notation "C ',' 'locals' x" :=
+Notation "C ',locals' x" :=
   (cons_locals C x)
   (at level 68, left associativity) : wasm_scope.
 
 
-(** functional update - prepend on fields *)
-
-Definition prepend_locals (C: context) (xs: list valtype) :=
-  {|
-    types := C.(types);
-    funcs := C.(funcs);
-    locals := xs ++ C.(locals);
-    labels := C.(labels);
-    return' := C.(return');
-  |}.
-Notation "C ',' 'locals__s' xs" :=
-  (prepend_locals C xs)
-  (at level 68, left associativity) : wasm_scope.
 
 (** Tests *)
 
@@ -127,54 +131,58 @@ Module ContextTests.
   Compute (nth 1 [1;2;3] 0).
   Compute (idx [1;2;3] 1).
 
-  Definition ex_C :=
+  Example ex_C :=
     {|
-      types := [];
-      funcs := [];
-      locals := [T_i32; T_i32];
-      labels := [];
-      return' := None;
+      C_types := [];
+      C_funcs := [];
+      C_tables := [];
+      C_locals := [T_i32; T_i32];
+      C_labels := [];
+      C_return := None;
     |}.
 
-  Compute (idx ex_C.(locals) 0).
-  Compute (idx ex_C.(locals) 1).
-  Compute (idx ex_C.(locals) 2).
+  Compute (idx ex_C.(C_locals) 0).
+  Compute (idx ex_C.(C_locals) 1).
+  Compute (idx ex_C.(C_locals) 2).
 
   (* Testing Updates Notation *)
-  Definition ex_C2 := ex_C with_labels = [[T_i32]].
-  Compute ex_C2.
+  Example ex_Crl := ex_C with_labels = [[T_i32]].
+  Compute ex_Crl.
 
-  Definition ex_Cr := ex_C with_return = [T_i32].
-  Compute ex_Cr.
+  Example ex_Crr := ex_C with_return = [T_i32].
+  Compute ex_Crr.
+
+  Example ex_Crlr := ex_C with_locals = [T_i32] with_return = [T_i32].
+  Compute ex_Crlr.
+
+  (* Testing if break pair *)
+  Example pair1 := (1,2).
+  Example pair2 := (1, 2).
 
   (* Testing Field Cons Notation *)
-  Definition ex_C3 := ex_C, labels [T_i32]. 
-  Compute ex_C3.
+  Example ex_Cc1 := ex_C,labels [T_i32]. 
+  Compute ex_Cc1.
 
-  Definition ex_C4 := ex_C, labels [T_f32], labels [T_i32]. 
-  Compute ex_C4.
+  Example ex_Cc2 := ex_C,labels [T_f32],labels [T_i32]. 
+  Compute ex_Cc2.
 
-  Definition ex_C5 := ex_C, locals__s [T_f32; T_f32].
-  Compute ex_C5.
-
-  Definition ex_C6 := ex_C, labels [T_f32], labels [T_i32] with_return = [T_i32].
-  Compute ex_C6.
-
-  Definition ex_C7 := ex_C, labels [T_f32], locals__s [T_i32; T_i32] with_return = [T_i32].
-  Compute ex_C7.
+  (* Testing associativity *)
+  Example ex_Ca1 := ex_C ,labels [T_f32] ,labels [T_i32] with_return = [T_i32].
+  Compute ex_Ca1.
 
   (* Testing Indexing Notation *)
   Compute ([1;2;3].[1] ).
 
-  Compute (ex_C.(locals).[0]).
-  Compute (ex_C.(locals).[1]).
-  Compute (ex_C.(locals).[2]).
+  Compute (ex_C.(C_locals).[0]).
+  Compute (ex_C.(C_locals).[1]).
+  Compute (ex_C.(C_locals).[2]).
 
-  Compute (forallb (fun ty => eqb_valtype ty T_i32) ex_C.(locals)).
-  Compute (all_valtype ex_C.(locals) T_i32).
+  Compute (forallb (fun ty => eqb_valtype ty T_i32) ex_C.(C_locals)).
+  Compute (all_valtype ex_C.(C_locals) T_i32).
 
   Check Forall.
-  Definition all_i32 := Forall (fun ty => ty = T_i32) (locals ex_C).
+  Example all_i32 := Forall (fun ty => ty = T_i32) (C_locals ex_C).
+
   Lemma ex_forall : all_i32.
   Proof with eauto.
     unfold all_i32.
@@ -190,25 +198,91 @@ End ContextTests.
 (** ** Types *)
 (** http://webassembly.github.io/spec/core/valid/types.html *)
 
+(* ----------------------------------------------------------------- *)
+(** *** Limits *)
+
+Reserved Notation "'⊢l' l '∈' k" (at level 70).
+Inductive valid_limit : limits -> I32.t -> Prop :=
+
+  (* No max limits *)
+
+  | VL__none: forall n k,
+      I32.le_u n k = true ->
+      ⊢l {| L_min := n; L_max := None |} ∈ k 
+
+  (* Has max limits *)
+       
+  | VL__some: forall n m k,
+      I32.le_u n k = true ->
+      I32.le_u m k = true ->
+      I32.le_u n m = true ->
+      ⊢l {| L_min := n; L_max := (Some m) |} ∈ k
+
+where "'⊢l' l '∈' k " := (valid_limit l k).
+
+Hint Constructors valid_limit.
+
+
+(* ----------------------------------------------------------------- *)
+(** *** Block Types *)
+(** https://webassembly.github.io/multi-value/core/valid/types.html#block-types *)
+
+(** Block types may be expressed in one of two forms, both of which are converted to plain function types by the following rules. *)
+
+Reserved Notation "C '⊢bt' bt '∈' ft" (at level 70).
+Inductive valid_blocktype : context -> blocktype -> functype -> Prop :=
+
+  | VBT_typeidx: forall C i ft,
+      C.(C_types).[i] = Some ft ->
+      C ⊢bt BT_typeidx i ∈ ft
+
+  | VBT_valtype__some: forall C t,
+      C ⊢bt BT_valtype (Some t) ∈ [] --> [t]
+
+  | VBT_valtype__none: forall C, 
+      C ⊢bt BT_valtype None ∈ [] --> []
+
+where "C '⊢bt' bt '∈' ft" := (valid_blocktype C bt ft).
+
 
 (* ----------------------------------------------------------------- *)
 (** *** Function Types *)
-(** http://webassembly.github.io/spec/core/valid/types.html#function-types *)
+(** https://webassembly.github.io/multi-value/core/valid/types.html#function-types *)
 
-(** The arity m must not be larger than 1.
-    The restriction to at most one result may be removed in future versions of WebAssembly.
- *)
 
 Reserved Notation "'⊢ft' ft 'ok'" (at level 70).
 Inductive valid_functype : functype -> Prop :=
+
   | VFT: forall ts1 ts2,
-      length ts2 <= 1 ->
       ⊢ft ts1 --> ts2 ok
+
 where "'⊢ft' ft 'ok' " := (valid_functype ft).
 
 Hint Constructors valid_functype.
 
 
+(* ----------------------------------------------------------------- *)
+(** *** Table Types *)
+
+Reserved Notation "'⊢tt' tt 'ok'" (at level 70).
+Inductive valid_tabletype : tabletype -> Prop :=
+
+  | VTT: forall limits elemtype,
+      ⊢l limits ∈ I32.max ->      (* spec use literal [2^32] here *)
+      ⊢tt (limits, elemtype) ok
+
+where "'⊢tt' tt 'ok' " := (valid_tabletype tt).
+
+Hint Constructors valid_tabletype.
+
+(* ----------------------------------------------------------------- *)
+(** *** Memory Types *)
+
+(* ----------------------------------------------------------------- *)
+(** *** Global Types *)
+
+(* ----------------------------------------------------------------- *)
+(** *** External Types *)
 
 
 (* ================================================================= *)
@@ -224,64 +298,71 @@ Hint Constructors valid_functype.
     off the operand stack and pushing new values of types [t2∗].
  *)
 
+
 Reserved Notation "C '⊢' instr '∈' ty" (at level 70).
-Reserved Notation "C '⊢s' instrs '∈' ty" (at level 70).
+Reserved Notation "C '⊢*' instrs '∈' ty" (at level 70).
+
 
 Inductive valid_instr : context -> instr -> functype -> Prop :=
 (* ----------------------------------------------------------------- *)
 (** *** Numeric Instruction *)
 
-  | VI_const : forall C t c,
-      C ⊢ const t c ∈ [] --> [t]
+  | VI_const : forall C t v,
+      t = type_of v ->
+      C ⊢ Const v ∈ [] --> [t]
 
-  | VI_iunop : forall C t op,
-      C ⊢ iunop t op ∈ [t] --> [t]
+  | VI_unop : forall C t op,
+      t = type_of op ->
+      C ⊢ Unop op ∈ [t] --> [t]
 
-  | VI_ibinop : forall C t op,
-      C ⊢ ibinop t op ∈ [t; t] --> [t]
+  | VI_binop : forall C t op,
+      t = type_of op ->
+      C ⊢ Binop op ∈ [t; t] --> [t]
 
-  | VI_itestop : forall C t op,
-      C ⊢ itestop t op ∈ [t] --> [T_i32]
+  | VI_testop : forall C t op,
+      t = type_of op ->
+      C ⊢ Testop op ∈ [t] --> [T_i32]
 
-  | VI_irelop : forall C t op,
-      C ⊢ irelop t op ∈ [t; t] --> [T_i32]
+  | VI_relop : forall C t op,
+      t = type_of op ->
+      C ⊢ Relop op ∈ [t; t] --> [T_i32]
 (*
   | VI_cvtop : forall C t1 t2 sx op,
-      C ⊢ cvtop t2 t1 sx op ∈ [t1] --> [t2]
+      C ⊢ Cvtop t2 t1 sx op ∈ [t1] --> [t2]
 *)
 
 (* ----------------------------------------------------------------- *)
 (** *** Parametric Instruction *)
 
   | VI_drop : forall C t,
-      C ⊢ drop ∈ [t] --> []
+      C ⊢ Drop ∈ [t] --> []
 
   | VI_select : forall C t,
-      C ⊢ select ∈ [t; t; T_i32] --> [t]
+      C ⊢ Select ∈ [t; t; T_i32] --> [t]
 
 (* ----------------------------------------------------------------- *)
 (** *** Variable Instruction *)
 
   | VI_local_get : forall C x t,
-      C.(locals).[x] = Some t ->
-      C ⊢ local_get x ∈ [] --> [t]
+      C.(C_locals).[x] = Some t ->
+      C ⊢ Local_get x ∈ [] --> [t]
 
   | VI_local_set : forall C x t,
-      C.(locals).[x] = Some t ->
-      C ⊢ local_set x ∈ [t] --> []
+      C.(C_locals).[x] = Some t ->
+      C ⊢ Local_set x ∈ [t] --> []
 
   | VI_local_tee : forall C x t,
-      C.(locals).[x] = Some t ->
-      C ⊢ local_tee x ∈ [t] --> [t]
+      C.(C_locals).[x] = Some t ->
+      C ⊢ Local_tee x ∈ [t] --> [t]
 
 (*
   | VI_global_get : forall C x t,
       C.(globals).[x] = Some t ->
-      C ⊢ global_get x ∈ [] --> [t]
+      C ⊢ Global_get x ∈ [] --> [t]
 
   | VI_global_set : forall C x t,
       C.(globals).[x] = Some t ->
-      C ⊢ global_set x ∈ [t] --> []
+      C ⊢ Global_set x ∈ [t] --> []
 *)
    
 (* ----------------------------------------------------------------- *)
@@ -291,50 +372,53 @@ Inductive valid_instr : context -> instr -> functype -> Prop :=
 (** *** Control Instructions *)
 
   | VI_nop : forall C,
-      C ⊢ nop ∈ [] --> []
+      C ⊢ Nop ∈ [] --> []
 
   | VI_unreachable : forall C ts1 ts2,
-      C ⊢ unreachable ∈ ts1 --> ts2
+      C ⊢ Unreachable ∈ ts1 --> ts2
 
-  | VI_block : forall C tr instrs,
-      C, labels tr ⊢s instrs ∈ [] --> tr ->
-      C ⊢ block tr instrs ∈ [] --> tr
+  | VI_block : forall C bt ts1 ts2 instrs,
+      C ⊢bt bt ∈ ts1 --> ts2 ->
+      C,labels ts2 ⊢* instrs ∈ ts1 --> ts2 ->
+      C ⊢ Block bt instrs ∈ ts1 --> ts2
 
-  | VI_loop : forall C tr instrs,
-      C, labels [] ⊢s instrs ∈ [] --> tr ->
-      C ⊢ loop tr instrs ∈ [] --> tr
+  | VI_loop : forall C bt ta tr instrs,
+      C ⊢bt bt ∈ ta --> tr ->
+      C,labels ta ⊢* instrs ∈ ta --> tr ->
+      C ⊢ Loop bt instrs ∈ ta --> tr
 
-  | VI_if : forall C tr instrs1 instrs2,
-      C, labels tr ⊢s instrs1 ∈ [] --> tr ->
-      C, labels tr ⊢s instrs2 ∈ [] --> tr ->
-      C ⊢ if' tr instrs1 instrs2 ∈ [T_i32] --> tr
+  | VI_if : forall C bt ta tr instrs1 instrs2,
+      C ⊢bt bt ∈ ta --> tr ->
+      C,labels tr ⊢* instrs1 ∈ ta --> tr ->
+      C,labels tr ⊢* instrs2 ∈ ta --> tr ->
+      C ⊢ If bt instrs1 instrs2 ∈ (ta ++ [T_i32]) --> tr
 
   | VI_br : forall C l tr ts1 ts2,
-      C.(labels).[l] = Some tr ->
-      C ⊢ br l ∈ (ts1 ++ tr) --> ts2
+      C.(C_labels).[l] = Some tr ->
+      C ⊢ Br l ∈ (ts1 ++ tr) --> ts2
 
   | VI_br_if : forall C l tr, 
-      C.(labels).[l] = Some tr ->
-      C ⊢ br_if l ∈ (tr ++ [T_i32]) --> tr
+      C.(C_labels).[l] = Some tr ->
+      C ⊢ Br_if l ∈ (tr ++ [T_i32]) --> tr
 
   | VI_br_table : forall C ls l__N tr ts1 ts2, 
       (* this might be easier via length check *)
-      Forall (fun l => C.(labels).[l] <> None) ls ->
-      C.(labels).[l__N] = Some tr ->
-      C ⊢ br_table ls l__N ∈ (ts1 ++ tr ++ [T_i32]) --> ts2
+      Forall (fun l => C.(C_labels).[l] <> None) ls ->
+      C.(C_labels).[l__N] = Some tr ->
+      C ⊢ Br_table ls l__N ∈ (ts1 ++ tr ++ [T_i32]) --> ts2
 
   | VI_return : forall C tr ts1 ts2,
-      C.(return') = Some tr ->
-      C ⊢ Structure.return' ∈ (ts1 ++ tr) --> ts2
+      C.(C_return) = Some tr ->
+      C ⊢ Return ∈ (ts1 ++ tr) --> ts2
 
   | VI_call : forall C x ts1 ts2,
-      C.(funcs).[x] = Some (ts1 --> ts2) ->
-      C ⊢ call x ∈ ts1 --> ts2
+      C.(C_funcs).[x] = Some (ts1 --> ts2) ->
+      C ⊢ Call x ∈ ts1 --> ts2
 
 (*
   | VI_call_indirect : forall C x ts1 ts2,
       C.(tables).[0] = ??? ->
-      C.(types).[x] = Some (ts1 --> ts2) ->
+      C.(C_types).[x] = Some (ts1 --> ts2) ->
       C ⊢ [call_indirect x] ∈ (ts1 ++ [i32]) --> ts2
 *)
 
@@ -344,15 +428,15 @@ Inductive valid_instr : context -> instr -> functype -> Prop :=
 
 with valid_seq : context -> list instr -> functype -> Prop :=
   | VIS_empty : forall C ts,
-      C ⊢s [] ∈ ts --> ts
+      C ⊢* [] ∈ ts --> ts
 
   | VIS_snoc : forall C instrs instr__N ts0 ts1 ts ts3,
       C ⊢ instr__N ∈ ts --> ts3 ->
-      C ⊢s instrs ∈ ts1 --> (ts0 ++ ts) ->
-      C ⊢s instrs ++ [instr__N] ∈ ts1 --> (ts0 ++ ts3)
+      C ⊢* instrs ∈ ts1 --> (ts0 ++ ts) ->
+      C ⊢* instrs ++ [instr__N] ∈ ts1 --> (ts0 ++ ts3)
 
 where "C '⊢' instr '∈' ty" := (valid_instr C instr ty)
-  and "C '⊢s' instrs '∈' ty" := (valid_seq C instrs ty).
+  and "C '⊢*' instrs '∈' ty" := (valid_seq C instrs ty).
 
 Hint Constructors valid_instr.
 Hint Constructors valid_seq.
@@ -377,7 +461,7 @@ Reserved Notation "C '⊢e' expr '∈' ty" (at level 70).
 Inductive valid_expr : context -> expr -> resulttype -> Prop :=
 
   | VE : forall C e tr,
-      C ⊢s e ∈ [] --> tr ->
+      C ⊢* e ∈ [] --> tr ->
       C ⊢e e ∈ tr
 
 where "C '⊢e' expr '∈' ty" := (valid_expr C expr ty).
@@ -405,8 +489,8 @@ Inductive const_expr : context -> expr -> Prop :=
 
 with const_instr : context -> instr -> Prop :=
 
-  | CI_const : forall C t c,
-      C ⊢ Structure.const t c const
+  | CI_const : forall C v,
+      C ⊢ Const v const
 
 where "C '⊢e' e 'const' " := (const_expr C e)
   and "C '⊢' instr 'const' " := (const_instr C instr).
@@ -435,48 +519,65 @@ Fixpoint check_expr (C : context) (e : expr) (tr : resulttype) :=
   * https://github.com/WebAssembly/spec/issues/1072
   *)
 
-Reserved Notation "C '⊢f' f ∈ ty" (at level 70).
+Reserved Notation "C '⊢f' f ∈ ft" (at level 70).
 Inductive valid_func : context -> func -> functype -> Prop :=
 
-  | VF : forall C (f: func) x ts expr ts1 ts2,
-      C.(types).[x] = Some (ts1 --> ts2) ->
-      C, locals__s (ts1 ++ ts), labels ts2 with_return = ts2 ⊢e expr ∈ ts2 ->
-      C ⊢f {| type := x; Structure.locals := ts; body := expr |} ∈ ts1 --> ts2
+  | VF : forall C x ts expr ts1 ts2,
+      C.(C_types).[x] = Some (ts1 --> ts2) ->
+      C with_locals = (ts1 ++ ts) with_labels = [ts2] with_return = ts2 ⊢e expr ∈ ts2 ->
+      C ⊢f {| F_type := x; F_locals := ts; F_body := expr |} ∈ ts1 --> ts2
 
-where "C '⊢f' f ∈ ty" := (valid_func C f ty).
+where "C '⊢f' f ∈ ft" := (valid_func C f ft).
 
-Definition ft := [T_i32] --> [T_i32].
-Definition ins :=
-  let '(ins --> outs) := ft in ins.
-Definition ins2 :=
-  match ft with
-  | (ins --> outs) => ins
-  end.
 
-Definition foo := Build_func 0 [] []. 
-Definition a :=
-  (* By let pattern *)
-  let 'Build_func a b c := foo in a.
-Definition a2 :=
-  (* By constructor pattern *)
-  match foo with
-    | Build_func a b c  => a
-  end.
-Definition a3 :=
-  (* By notational pattern *)
-  match foo with
-    | {| type := a; Structure.locals := b; body := c |} => a
-  end.
+Module FuncTyTest.
+
+  Definition ft := [T_i32] --> [T_i32].
+  Definition ins :=
+    let '(ins --> outs) := ft in ins.
+  Definition ins2 :=
+    match ft with
+    | (ins --> outs) => ins
+    end.
+
+  Definition foo := Build_func 0 [] []. 
+  Definition a :=
+    (* By let pattern *)
+    let 'Build_func a b c := foo in a.
+  Definition a2 :=
+    (* By constructor pattern *)
+    match foo with
+      | Build_func a b c  => a
+    end.
+  Definition a3 :=
+    (* By notational pattern *)
+    match foo with
+      | {| F_type := a; F_locals := b; F_body := c |} => a
+    end.
+
+End FuncTyTest.
 
 (* postpone functional type checking.
 
 Fixpoint check_func (C: context) (f: func) :=
   let '(Build_func type locals body) := f in
-  let '(ts1 --> ts2) := C.(types).[type] in
+  let '(ts1 --> ts2) := C.(C_types).[type] in
   let C' = C, locals__s (ts1 ++ ts), labels ts2 with_return = ts2 in
   check_expr C' body ts2.
 *)
 
+
+(* ----------------------------------------------------------------- *)
+(** *** Tables *)
+
+Reserved Notation "C '⊢t' t ∈ tt" (at level 70).
+Inductive valid_table : context -> table -> tabletype -> Prop :=
+
+  | VT : forall C tablety,
+      ⊢tt tablety ok ->
+      C ⊢t {| T_type := tablety |} ∈ tablety
+
+where "C '⊢t' t ∈ tt" := (valid_table C t tt).
 
 
 (* ----------------------------------------------------------------- *)
@@ -489,30 +590,36 @@ Fixpoint check_func (C: context) (f: func) :=
 (** Let ft∗ be the concatenation of the internal function types fti, in index order.
  *)
 
-
-Reserved Notation "'⊢' module ∈ ty" (at level 70).
+Reserved Notation "'⊢' M ∈ ty" (at level 70).
 Inductive valid_module: module -> functype -> Prop :=
-  | VM : forall (m: module) its ets fts ft,
+  | VM : forall M its ets fts ts,
       let
-        C : context := {|
-          types := m.(Structure.types);
-          funcs := fts;
-          locals := [];
-          labels := [];
-          return' := None;
+        C := {|
+          C_types := M.(M_types);
+          C_funcs := fts;
+          C_tables := ts;
+          C_locals := [];
+          C_labels := [];
+          C_return := None;
         |}
       in
-      Forall (fun functype => ⊢ft functype ok) m.(Structure.types) ->
-      Forall (fun func => C ⊢f func ∈ ft) m.(Structure.funcs) ->
-      ⊢ m ∈ its --> ets
+      (* this has been removed in multi-value *)
+      Forall (fun functype => ⊢ft functype ok) M.(M_types) ->
+
+      (* pairwise related *)
+      Forall2 (fun func ft => C ⊢f func ∈ ft) M.(M_funcs) fts ->  
+
+      Forall (fun table => C ⊢t table ∈ table.(T_type)) M.(M_tables) ->
+
+      ⊢ M ∈ its --> ets
       
-where "'⊢' m ∈ ty" := (valid_module m ty).
+where "'⊢' M ∈ ty" := (valid_module M ty).
 
 
 (* postpone functional type checking.
 
 Fixpoint prepass_funcs (funcs : list func) : list functype :=
-  map (fun func => C.(types).[func.type]) funcs. 
+  map (fun func => C.(C_types).[func.type]) funcs. 
 
 Fixpoint check_module 
 
