coq/Commons.v
@@ -1,0 +1,114 @@
+(* ***************************************************************** *)
+(* Commons.v                                                         *)
+(*                                                                   *)
+(* 2019 Xuan Huang                                                   *)
+(* ***************************************************************** *)
+
+From Coq Require Export Lists.List.
+Export ListNotations.
+
+(* ################################################################# *)
+(** * Commons *)
+
+(* ================================================================= *)
+(** ** Notations *)
+
+(* ----------------------------------------------------------------- *)
+(** *** Epsilon *)
+Notation " 'ϵ' " := ([]).
+
+(* ----------------------------------------------------------------- *)
+(** *** Indexing *)
+
+Module IndexingNotations.
+
+  Notation idx := nth_error.
+
+  Notation "l '.[' x ]" :=
+    (idx l x)
+    (at level 60, right associativity) : wasm_scope.
+
+  Open Scope wasm_scope.
+
+  Fixpoint update_idx {A: Type} (l: list A) (n: nat) (x: A) : option (list A) :=
+    match l.[n] with
+    | None => None
+    | Some _ => Some ((firstn n l) ++ [x] ++ (skipn (n+1) l))
+    end.
+
+  Module Test.
+
+    Example l := [1;2;3].
+
+    Example i0 : (update_idx l 0 2) = Some [2;2;3].
+      auto. Qed.
+
+    Example i1 : (update_idx l 1 4) = Some [1;4;3].
+      auto. Qed.
+
+    Example i__overflow : (update_idx l 3 4) = None.
+      auto. Qed.
+
+  End Test.
+
+End IndexingNotations.
+Export IndexingNotations.
+
+
+
+(* ================================================================= *)
+(** ** Monads *)
+
+(* ----------------------------------------------------------------- *)
+(** *** Monadaic/Fmap option *)
+
+Module OptionMonadNotations.
+
+  Notation "x <- e1 ;; e2" := (match e1 with
+                                | Some x => e2
+                                | None => None
+                                end)
+           (right associativity, at level 60) : option_scope.
+
+  Notation " 'return' e "
+    := (Some e) (at level 60) : option_scope.
+
+  Notation " 'fail' "
+    := None : option_scope.
+
+
+  Definition fmap_opt {A B: Type} (f: A -> B) (o1: option A) : option B :=
+    match o1 with
+    | Some x => Some (f x)
+    | None => None
+    end.
+
+  Notation " f '<$>' o "
+    := (fmap_opt f o) (right associativity, at level 60) : option_scope.
+
+  Open Scope option_scope.
+
+  Module Test.
+
+    Example exf :=  (fun i => i + 1) <$> (Some 0).
+    Compute exf.
+
+    Example exf__assoc := (fun i => i + 1) <$> (fun i => i + 1) <$> (Some 0).
+    Compute exf__assoc.
+
+    Example exm__some :=
+      v1 <- Some 1;;
+      v2 <- Some 2;;
+      return (v1 + v2).
+    Compute exm__some.
+
+    Example exm__none :=
+      v1 <- Some 1;;
+      v2 <- None;;
+      return (v1 + v2).
+    Compute exm__none.
+
+  End Test.
+
+End OptionMonadNotations.
+Export OptionMonadNotations.
