coq/Float.v
@@ -1,0 +1,111 @@
+
+(* ***************************************************************** *)
+(* Float.v                                                           *)
+(*                                                                   *)
+(* 2019 Xuan Huang                                                   *)
+(* ***************************************************************** *)
+
+
+(* ################################################################# *)
+(** * Float  *)
+
+(* ----------------------------------------------------------------- *)
+(** *** Value representation (placeholder) *)
+
+(** TODO: use actual implementation such as Coq standard library's
+    or Int32, Int64, Float32, Float64 from OCaml.
+ *)
+
+Module Type Rep.
+  Parameter bitwidth: nat.
+End Rep.
+
+Module Rep32.
+  Definition bitwidth := 32.
+End Rep32.
+
+Module Rep64.
+  Definition bitwidth := 64.
+End Rep64.
+
+
+(* ----------------------------------------------------------------- *)
+(** *** Functor *)
+
+Module Type S.
+  Parameter t : Type.
+  Parameter bitwidth: nat.
+
+  Parameter zero : t.
+
+  (* funop *)
+  Parameter abs : t -> option t.
+  Parameter neg : t -> option t.
+  Parameter sqrt : t -> option t.
+  Parameter ceil : t -> option t.
+  Parameter floor : t -> option t.
+  Parameter trunc : t -> option t.
+  Parameter nearest : t -> option t.
+
+  (* fbinop *)
+  Parameter add : t -> t -> option t.
+  Parameter sub : t -> t -> option t.
+  Parameter mul : t -> t -> option t.
+  Parameter div : t -> t -> option t.
+  Parameter min : t -> t -> option t.
+  Parameter max : t -> t -> option t.
+  Parameter copysign : t -> t -> option t.
+
+  (* fretop *)
+  Parameter eq : t -> t -> bool.
+  Parameter ne : t -> t -> bool.
+  Parameter lt : t -> t -> bool.
+  Parameter gt : t -> t -> bool.
+  Parameter le : t -> t -> bool.
+  Parameter ge : t -> t -> bool.
+
+  (* axioms *)
+End S.
+
+Module Make (R: Rep) : S.
+  Include R.
+
+  Parameter t : Type.
+
+  Parameter zero : t.
+
+  (* funop *)
+  Parameter abs : t -> option t.
+  Parameter neg : t -> option t.
+  Parameter sqrt : t -> option t.
+  Parameter ceil : t -> option t.
+  Parameter floor : t -> option t.
+  Parameter trunc : t -> option t.
+  Parameter nearest : t -> option t.
+
+  (* fbinop *)
+  Parameter add : t -> t -> option t.
+  Parameter sub : t -> t -> option t.
+  Parameter mul : t -> t -> option t.
+  Parameter div : t -> t -> option t.
+  Parameter min : t -> t -> option t.
+  Parameter max : t -> t -> option t.
+  Parameter copysign : t -> t -> option t.
+
+  (* fretop *)
+  Parameter eq : t -> t -> bool.
+  Parameter ne : t -> t -> bool.
+  Parameter lt : t -> t -> bool.
+  Parameter gt : t -> t -> bool.
+  Parameter le : t -> t -> bool.
+  Parameter ge : t -> t -> bool.
+
+  (* axioms *)
+End Make.
+
+
+(* ----------------------------------------------------------------- *)
+(** *** Make *)
+
+Module F32 := Float.Make(Rep32).
+Module F64 := Float.Make(Rep64).
