coq/Int.v
@@ -1,0 +1,146 @@
+
+(* ***************************************************************** *)
+(* Int.v                                                             *)
+(*                                                                   *)
+(* 2019 Xuan Huang                                                   *)
+(* ***************************************************************** *)
+
+
+(* ################################################################# *)
+(** * Int  *)
+
+(* ----------------------------------------------------------------- *)
+(** *** Value representation (placeholder) *)
+
+(** TODO: use actual implementation such as Coq standard library's
+    or Int32, Int64, Float32, Float64 from OCaml.
+ *)
+
+Module Type Rep.
+  Parameter bitwidth: nat.
+End Rep.
+
+Module Rep32.
+  Definition bitwidth := 32.
+End Rep32.
+
+Module Rep64.
+  Definition bitwidth := 64.
+End Rep64.
+
+
+(* ----------------------------------------------------------------- *)
+(** *** Functor *)
+
+Module Type S.
+  Parameter t : Type.
+  Parameter bitwidth: nat.
+
+  Parameter zero : t.
+  Parameter one : t.
+  Parameter min : t.
+  Parameter max : t.
+
+  Parameter from_nat : nat -> t.
+  Parameter to_nat : t -> nat.
+
+  (* iunop *)
+  Parameter clz    : t -> option t.
+  Parameter ctz    : t -> option t.
+  Parameter popcnt : t -> option t.
+
+  (* ibinop *)
+  Parameter add   : t -> t -> option t.
+  Parameter sub   : t -> t -> option t.
+  Parameter mul   : t -> t -> option t.
+  Parameter div_s : t -> t -> option t.
+  Parameter div_u : t -> t -> option t.
+  Parameter rem_s : t -> t -> option t.
+  Parameter rem_u : t -> t -> option t.
+  Parameter and   : t -> t -> option t.
+  Parameter or    : t -> t -> option t.
+  Parameter xor   : t -> t -> option t.
+  Parameter shl   : t -> t -> option t.
+  Parameter shr_s : t -> t -> option t.
+  Parameter shr_u : t -> t -> option t.
+  Parameter rotl  : t -> t -> option t.
+  Parameter rotr  : t -> t -> option t.
+
+  (* itestop *)
+  Parameter eqz : t -> bool.
+
+  (* iretop *)
+  Parameter eq   : t -> t -> bool.
+  Parameter ne   : t -> t -> bool.
+  Parameter lt_s : t -> t -> bool.
+  Parameter lt_u : t -> t -> bool.
+  Parameter gt_s : t -> t -> bool.
+  Parameter gt_u : t -> t -> bool.
+  Parameter le_s : t -> t -> bool.
+  Parameter le_u : t -> t -> bool.
+  Parameter ge_s : t -> t -> bool.
+  Parameter ge_u : t -> t -> bool.
+
+  (* axioms *)
+End S.
+
+
+Module Make (R: Rep) : S.
+  Include R.
+
+  Parameter t : Type.
+
+  Parameter zero : t.
+  Parameter one : t.
+  Parameter min : t.
+  Parameter max : t.
+
+  Parameter from_nat : nat -> t.
+  Parameter to_nat : t -> nat.
+
+  (* iunop *)
+  Parameter clz    : t -> option t.
+  Parameter ctz    : t -> option t.
+  Parameter popcnt : t -> option t.
+
+  (* ibinop *)
+  Parameter add   : t -> t -> option t.
+  Parameter sub   : t -> t -> option t.
+  Parameter mul   : t -> t -> option t.
+  Parameter div_s : t -> t -> option t.
+  Parameter div_u : t -> t -> option t.
+  Parameter rem_s : t -> t -> option t.
+  Parameter rem_u : t -> t -> option t.
+  Parameter and   : t -> t -> option t.
+  Parameter or    : t -> t -> option t.
+  Parameter xor   : t -> t -> option t.
+  Parameter shl   : t -> t -> option t.
+  Parameter shr_s : t -> t -> option t.
+  Parameter shr_u : t -> t -> option t.
+  Parameter rotl  : t -> t -> option t.
+  Parameter rotr  : t -> t -> option t.
+
+  (* itestop *)
+  Parameter eqz : t -> bool.
+
+  (* iretop *)
+  Parameter eq   : t -> t -> bool.
+  Parameter ne   : t -> t -> bool.
+  Parameter lt_s : t -> t -> bool.
+  Parameter lt_u : t -> t -> bool.
+  Parameter gt_s : t -> t -> bool.
+  Parameter gt_u : t -> t -> bool.
+  Parameter le_s : t -> t -> bool.
+  Parameter le_u : t -> t -> bool.
+  Parameter ge_s : t -> t -> bool.
+  Parameter ge_u : t -> t -> bool.
+
+  (* axioms *)
+End Make.
+
+
+(* ----------------------------------------------------------------- *)
+(** *** Make *)
+
+Module I32 := Int.Make(Rep32).
+Module I64 := Int.Make(Rep64).
