coq/Numerics.v
@@ -1,0 +1,284 @@
+(* ***************************************************************** *)
+(* Numerics.v                                                       *)
+(*                                                                   *)
+(* 2019 Xuan Huang                                                   *)
+(* ***************************************************************** *)
+
+
+(* ################################################################# *)
+(** * Numerics *)
+
+From Wasm Require Export Values.
+From Wasm Require Export Structure.
+
+Module S := Structure.
+
+(* ================================================================= *)
+(** * Runtime Type Error (Stuck) *)
+
+Inductive runtime_err (X:Type) : Type :=
+  | Ok (x : X)
+  | Err.
+
+Arguments Ok {X} _.
+Arguments Err {X}.
+
+
+
+(* ================================================================= *)
+(** * Int Operator *)
+
+(* took me a while to find the syntax of module shared constraints: 
+   https://coq.inria.fr/refman/language/gallina-extensions.html#module-system
+ *)
+
+Module IntOp (IXX : Int.S) (Val : ValType with Definition t := IXX.t). 
+
+  Import S.IntOp.
+
+  Definition to_val := Val.to_val.
+  Definition of_val := Val.of_val.
+
+  Definition unop op : (val -> runtime_err (option val)) :=
+    let f :=
+      match op with
+      | Clz => IXX.clz
+      | Ctz => IXX.ctz
+      | Popcnt => IXX.popcnt
+      end
+    in
+    fun (v : val) =>
+      match of_val v with
+      | Some i1 => Ok (to_val <$> f i1)
+      | None => Err
+      end.
+
+
+  Definition binop op : (val -> val -> runtime_err (option val)) :=
+    let f :=
+      match op with
+      | Add => IXX.add
+      | Sub => IXX.sub
+      | Mul => IXX.mul
+      | Div sx =>
+        match sx with
+        | U => IXX.div_u
+        | S => IXX.div_s
+        end
+      | Rem sx =>
+        match sx with
+        | U => IXX.rem_u
+        | S => IXX.rem_s
+        end
+      | And => IXX.and
+      | Or => IXX.or
+      | Xor => IXX.xor
+      | Shl => IXX.shl
+      | Shr sx =>
+        match sx with
+        | U => IXX.shr_u
+        | S => IXX.shr_s
+        end
+      | Rotl => IXX.rotl
+      | Rotr => IXX.rotr
+      end
+    in
+    fun (v1 v2 : val) =>
+      match of_val v1, of_val v2 with
+      | Some i1, Some i2 => Ok (to_val <$> f i1 i2)
+      | _, _ => Err
+      end.
+
+
+  Definition testop op : (val -> runtime_err bool) :=
+    let f :=
+      match op with
+      | Eqz => IXX.eqz
+      end
+    in
+    fun (v : val) =>
+      match of_val v with
+      | Some i => Ok (f i)
+      | None => Err
+      end.
+      
+
+  Definition relop op : (val -> val -> runtime_err bool) :=
+    let f :=
+      match op with
+      | Eq => IXX.eq
+      | Ne => IXX.ne
+      | Lt sx =>
+        match sx with
+        | U => IXX.lt_s
+        | S => IXX.lt_u
+        end
+      | Le sx =>
+        match sx with
+        | U => IXX.le_s
+        | S => IXX.le_u
+        end
+      | Gt sx =>
+        match sx with
+        | U => IXX.gt_s
+        | S => IXX.gt_u
+        end
+      | Ge sx =>
+        match sx with
+        | U => IXX.ge_s
+        | S => IXX.ge_u
+        end
+      end
+    in
+    fun (v1 v2 : val) =>
+      match of_val v1, of_val v2 with
+      | Some i1, Some i2 => Ok (f i1 i2)
+      | _, _ => Err
+      end.
+
+End IntOp. 
+
+Module IOp32 := IntOp (I32) (IVal32).
+Module IOp64 := IntOp (I64) (IVal64).
+
+
+
+(* ================================================================= *)
+(** * Float Operator *)
+
+
+Module FloatOp (FXX : Float.S) (Val : ValType with Definition t := FXX.t). 
+
+  Import S.FloatOp.
+
+  Definition to_val := Val.to_val.
+  Definition of_val := Val.of_val.
+
+  Definition unop op : (val -> runtime_err (option val)) :=
+    let f :=
+      match op with
+      | Neg => FXX.neg
+      | Abs => FXX.abs
+      | Sqrt => FXX.sqrt
+      | Ceil => FXX.ceil
+      | Floor => FXX.floor
+      | Trunc => FXX.trunc
+      | Nearest => FXX.nearest
+      end
+    in
+    fun (v : val) =>
+      match of_val v with
+      | Some f1 => Ok (to_val <$> f f1)
+      | None => Err
+      end.
+      
+
+  Definition binop op : (val -> val -> runtime_err (option val)) :=
+    let f :=
+      match op with
+      | Add => FXX.add
+      | Sub => FXX.sub
+      | Mul => FXX.mul
+      | Div => FXX.div
+      | Min => FXX.min
+      | Max => FXX.max
+      | Copysign => FXX.copysign
+      end
+    in
+    fun (v1 v2 : val) =>
+      match of_val v1, of_val v2 with
+      | Some f1, Some f2 => Ok (to_val <$> f f1 f2)
+      | _, _ => Err
+      end.
+  
+
+  Definition testop (op : testop) : (val -> runtime_err bool) :=
+    fun v => Err.
+      
+
+  Definition relop op : (val -> val -> runtime_err bool) :=
+    let f :=
+      match op with
+      | Eq => FXX.eq
+      | Ne => FXX.ne
+      | Lt => FXX.lt
+      | Le => FXX.le
+      | Gt => FXX.gt
+      | Ge => FXX.ge
+      end
+    in
+    fun (v1 v2 : val) =>
+      match of_val v1, of_val v2 with
+      | Some f1, Some f2 => Ok (f f1 f2)
+      | _, _ => Err
+      end.
+
+End FloatOp. 
+
+Module FOp32 := FloatOp (F32) (FVal32).
+Module FOp64 := FloatOp (F64) (FVal64).
+
+
+(** Dispatch *)
+
+Definition eval_unop (ops: @op S.IntOp.unop S.IntOp.unop S.FloatOp.unop S.FloatOp.unop) := 
+  match ops with
+  | i32 x => IOp32.unop x
+  | i64 x => IOp64.unop x
+  | f32 x => FOp32.unop x
+  | f64 x => FOp64.unop x
+  end.
+
+
+Definition eval_binop (ops: @op S.IntOp.binop S.IntOp.binop S.FloatOp.binop S.FloatOp.binop) :=
+  match ops with
+  | i32 x => IOp32.binop x
+  | i64 x => IOp64.binop x
+  | f32 x => FOp32.binop x
+  | f64 x => FOp64.binop x
+  end.
+
+Definition eval_testop (ops: @op S.IntOp.testop S.IntOp.testop S.FloatOp.testop S.FloatOp.testop) :=
+  match ops with
+  | i32 x => IOp32.testop x
+  | i64 x => IOp64.testop x
+  | f32 x => FOp32.testop x
+  | f64 x => FOp64.testop x
+  end.
+
+Definition eval_relop (ops: @op S.IntOp.relop S.IntOp.relop S.FloatOp.relop S.FloatOp.relop) :=
+  match ops with
+  | i32 x => IOp32.relop x
+  | i64 x => IOp64.relop x
+  | f32 x => FOp32.relop x
+  | f64 x => FOp64.relop x
+  end.
+
+(* post pone convertion op
+
+Definition eval_cvtop (ops: @op S.IntOp.cvtop S.IntOp.cvtop S.FloatOp.cvtop S.FloatOp.cvtop) :=
+  match ops with
+  | i32 x => IOp32.cvtop x
+  | i64 x => IOp64.cvtop x
+  | f32 x => FOp32.cvtop x
+  | f64 x => FOp64.cvtop x
+  end.
+
+*)
+
+
+(*  not sure how to write the generic function...
+
+Definition eval_op iop32 iop64 fop32 fop64 :=
+  fun {i32 i64 f32 f64 : Type} (ops : op i32 i64 f32 f64) =>
+  match ops with
+  | i32 x => iop32 x
+  | i64 x => iop64 x
+  | f32 x => fop32 x
+  | f64 x => fop64 x
+  end. 
+
+Definition eval_unop := eval_op S.IntOp.unop S.IntOp.unop S.FloatOp.unop S.FloatOp.unop.
+
+*)
+
