coq/Types.v
@@ -1,0 +1,226 @@
+(* ***************************************************************** *)
+(* Types.v                                                           *)
+(*                                                                   *)
+(* 2019 Xuan Huang                                                   *)
+(* ***************************************************************** *)
+
+
+(* ################################################################# *)
+(** * Types *)
+
+(* It's interesting that if we use
+
+     Require Export Int.
+     Require Export Float.
+
+   Here, we will later hit errors in [Execution.v] saying:
+ 
+     (cannot unify "I32.t" and "Values.I32.t").
+
+   This might be a bug or intentional of Coq.
+   Issue posted: https://github.com/coq/coq/issues/10869
+ *)
+From Wasm Require Import Int.
+From Wasm Require Import Float.
+From Coq Require Export Lists.List.
+Export ListNotations.
+
+(* ----------------------------------------------------------------- *)
+(** *** Value Types *)
+
+Inductive valtype :=
+  | T_i32
+  | T_i64
+  | T_f32
+  | T_f64.
+
+Definition eqb_valtype (ty1 ty2: valtype) : bool :=
+  match ty1, ty2 with
+  | T_i32, T_i32 => true
+  | T_i64, T_i64 => true
+  | T_f32, T_f32 => true
+  | T_f64, T_f64 => true
+  | _, _ => false
+  end.
+
+Definition all_valtype (ts: list valtype) (t': valtype) :=
+  forallb (fun t => eqb_valtype t t') ts.
+
+Lemma eqb_valtype_refl : forall (ty: valtype),
+  eqb_valtype ty ty = true.
+Proof.
+  destruct ty; auto.
+Qed.
+
+Lemma eqb_valtype_eq : forall (ty1 ty2: valtype),
+  eqb_valtype ty1 ty2 = true -> ty1 = ty2.
+Proof with eauto.
+  intro ty1.
+  destruct ty1;
+    intros ty2 Heqb;
+    destruct ty2; inversion Heqb...
+Qed.
+
+(** Having eq_dec is equivalent to having eqb and its spec
+    How? https://coq.inria.fr/library/Coq.Structures.Equalities.html
+  *)
+Lemma valtype_eq_dec: forall (ty1 ty2: valtype), {ty1 = ty2} + {ty1 <> ty2}.
+Proof.
+  decide equality.
+Qed.
+
+
+Module TestValtypeEq.
+
+  Compute (all_valtype [T_i32] T_i32).
+
+  Example ex1 (ty: valtype) := if valtype_eq_dec ty T_i32 then true else false.
+
+  Compute (ex1 T_i32).
+
+  Lemma ex2: ex1(T_i32) = true.
+  Proof.
+    Abort.
+
+
+End TestValtypeEq.
+  
+
+(* ----------------------------------------------------------------- *)
+(** *** Result Types *)
+
+(** the current spec use optional occurence such as
+
+      Definition resulttype : Type := option valtype.
+
+    while we moved to the "multi-value" proposal where
+
+      resulttype ::= [vec(valtype)]
+
+    See option valtype section below.
+ *)
+
+Notation resulttype := (list valtype). 
+
+
+
+(* ----------------------------------------------------------------- *)
+(** *** Function Types *)
+
+Record functype :=
+  {
+    ins : resulttype;
+    outs: resulttype;
+  }.
+
+Module FunctypeNotations.
+
+  Notation "ts1 --> ts2" :=
+    ({| ins := ts1; outs := ts2|})
+    (at level 30, right associativity) : wasm_scope.
+  Open Scope wasm_scope.
+
+End FunctypeNotations.
+
+
+(** Testing *)
+
+Module TypesTest.
+
+  Example ex_res1: resulttype := [].
+  Example ex_res2: resulttype := [T_i32].
+  Example ex_fun: functype := {| ins := [T_i32]; outs := [T_i32] |}.
+
+  (* Func Notation Testing *)
+
+  Import FunctypeNotations.
+
+  Example ex_fun_nu : functype := [] --> [T_i32].
+  Compute ex_fun_nu.
+
+  Example ex_fun_un : functype := [T_i32] --> [T_i32].
+  Compute ex_fun_un.
+
+  Example ex_fun_bin : functype := [T_i32; T_i32] --> [T_i32].
+  Compute ex_fun_bin.
+
+  (* cannot looser than ++ *)
+  Example ex_fun_loose : functype := ([T_i32] ++ [T_i32]) --> [T_i32].
+
+End TypesTest.
+
+
+(* ----------------------------------------------------------------- *)
+(** *** Limits *)
+
+(* techinically the spec use [u32], which mean we should interpter
+   this [I32.t] as unsigned integers. *)
+
+Record limits := 
+  {
+    L_min: Int.I32.t;
+    L_max: option Int.I32.t;
+  }.
+
+(* ----------------------------------------------------------------- *)
+(** *** Memory Types *)
+
+Definition memtype := limits.
+
+
+(* ----------------------------------------------------------------- *)
+(** *** Table Types *)
+
+(* according to spec:
+
+   > The element type [funcref] is the infinite union of all function types.
+     A table of that type thus contains references to functions of
+     heterogeneous type.
+
+   the [Call_indirect] will fetch index into this table,
+   and the type of function is **checked dynamically**
+
+   combined it can represent *function pointer* and dynamic linking.
+ *)
+
+Inductive elemtype := funcref.
+
+Definition tabletype : Type := limits * elemtype.
+
+
+(* ----------------------------------------------------------------- *)
+(** *** Global Types *)
+
+
+(* ----------------------------------------------------------------- *)
+(** *** External Types *)
+
+
+(* ----------------------------------------------------------------- *)
+(** *** Option ValType Occurence *)
+
+(* Not currently used in favor of plain [option value]
+   Potential uses would be [blocktype] and module [M_return].
+ *)
+
+Definition opt_valtype := (option valtype).
+
+Definition opt_to_rt (opt : opt_valtype) : resulttype :=
+  match opt with
+  | Some valtype => [valtype]
+  | None => []
+  end.
+
+Coercion opt_to_rt : opt_valtype >-> resulttype.
+
+Module OptionValTyTest.
+
+  Import FunctypeNotations.
+
+  Example valtype1 : opt_valtype := Some T_i32.
+  Example valtype2 : opt_valtype := None.
+
+  Example ft_some := [] --> opt_to_rt valtype1.
+  Example ft_some2 := [] --> valtype1.
+
+End OptionValTyTest.
