coq/Values.v
@@ -1,0 +1,194 @@
+
+(* ***************************************************************** *)
+(* Values.v                                                          *)
+(*                                                                   *)
+(* 2019 Xuan Huang                                                   *)
+(* ***************************************************************** *)
+
+
+(* ################################################################# *)
+(** * Values  *)
+
+From Wasm Require Export Int.
+From Wasm Require Export Float.
+From Wasm Require Export Types.
+
+
+(* ================================================================= *)
+(** ** Structure - Value *)
+
+(** Definied in [Int.v] and [Float.v] *)
+
+Module ValRepTest.
+
+  Definition should_be_32 := I32.bitwidth.
+
+End ValRepTest.
+
+
+(* ----------------------------------------------------------------- *)
+(** *** Bytes *)
+
+Parameter byte : Type.
+
+
+(* ================================================================= *)
+(** ** Execution - Runtime Structure - Values *)
+
+(** From the reference interpter...
+    Module and constructors use different namespace:
+
+        type ('i32, 'i64, 'f32, 'f64) op =
+          I32 of 'i32 | I64 of 'i64 | F32 of 'f32 | F64 of 'f64
+
+        type value = (I32.t, I64.t, F32.t, F64.t) op
+
+    But here in Coq we can start constructor name in lowercase anyway.
+ *)
+
+
+(* op is a sum that representing any 4-ways things *)
+
+Inductive op (i32 i64 f32 f64 : Type) :=
+  | i32 (_: i32)
+  | i64 (_: i64)
+  | f32 (_: f32)
+  | f64 (_: f64).
+Arguments i32 {i32} {i64} {f32} {f64} _.
+Arguments i64 {i32} {i64} {f32} {f64} _.
+Arguments f32 {i32} {i64} {f32} {f64} _.
+Arguments f64 {i32} {i64} {f32} {f64} _.
+
+
+(* wasm vals is sum of 4 concrete rep value. *)
+
+Definition val := op I32.t I64.t F32.t F64.t.
+
+
+(* functor map ops to wasm types. *)
+
+Definition type_of {i32 i64 f32 f64 : Type} (ops : op i32 i64 f32 f64) : valtype :=
+  match ops with
+  | i32 _ => T_i32
+  | i64 _ => T_i64
+  | f32 _ => T_f32
+  | f64 _ => T_f64
+  end.
+
+(* map [valtype*] to corresponding zeros *)
+
+Definition zeros (ts: list valtype) : list val :=
+  map (fun t => match t with
+           | T_i32 => i32 I32.zero
+           | T_i64 => i64 I64.zero
+           | T_f32 => f32 F32.zero
+           | T_f64 => f64 F64.zero
+         end) ts.
+
+
+(* functor map ops to concrete rep's coq type. *)
+
+Definition rep_type_of {i32 i64 f32 f64 : Type} (ops : op i32 i64 f32 f64) : Type :=
+  match ops with
+  | i32 _ => I32.t
+  | i64 _ => I64.t
+  | f32 _ => F32.t
+  | f64 _ => F64.t
+  end.
+
+
+(* bool is represented as i32 *)
+
+Definition bool_to_i32 (b : bool) : val :=
+  match b with
+  | true => i32 I32.one
+  | false => i32 I32.zero
+  end.
+Coercion bool_to_i32 : bool >-> val.
+
+
+(* nat is used to index vector *)
+
+Definition nat_to_i32 (n : nat) : val :=
+  match n with
+  | 0 => i32 I32.zero
+  | n => i32 (I32.from_nat n)
+  end.
+Coercion nat_to_i32 : nat >-> val.
+
+
+Module ValTest.
+
+  Parameter c32 : I32.t.
+  Definition c64 := I64.zero.
+
+  Example v1: val := i32 c32.
+  Compute v1.
+  Compute (rep_type_of v1).
+
+  Example v2 : val := i64 (I64.zero).
+  Compute v2.
+
+  Example vb: val := true.
+  Compute vb.
+
+  Fail Example v3 := I32 c64.
+
+End ValTest.
+
+
+
+(* ================================================================= *)
+(** ** Injection & Projection *)
+
+(** the reference interpreter simly raise exception here but here we have to make the conversion exception explicit. *)
+
+Module Type ValType.
+  Parameter t : Type.
+  Parameter to_val : t -> val.
+  Parameter of_val : val -> option t.
+End ValType.
+
+
+Module IVal32.
+  Definition t := I32.t.
+  Definition to_val i : val := i32 i.
+  Definition of_val (v: val) :=
+    match v with
+    | i32 i => Some i
+    | _ => None
+    end.
+End IVal32.
+
+
+Module IVal64.
+  Definition t := I64.t.
+  Definition to_val i : val := i64 i.
+  Definition of_val (v: val) :=
+    match v with
+    | i64 i => Some i
+    | _ => None
+    end.
+End IVal64.
+
+
+Module FVal32.
+  Definition t := F32.t.
+  Definition to_val f : val := f32 f.
+  Definition of_val (v: val) :=
+    match v with
+    | f32 f => Some f
+    | _ => None
+    end.
+End FVal32.
+
+
+Module FVal64.
+  Definition t := F64.t.
+  Definition to_val f : val := f64 f.
+  Definition of_val (v: val) :=
+    match v with
+    | f64 f => Some f
+    | _ => None
+    end.
+End FVal64.
