doc/eng-note.md
@@ -36,12 +36,30 @@ The coq formalization need to:
 - explicity option type: `Some` and `None` are treat as subsumption rather than disjointed. `resulttype` could implicitly be a `Some resulttype`. and `[]` could be either `None` or `nil`
 
 
-About `resultype`
------------------
+On the use of `resultype`
+-------------------------
 
-[spec - Should functions return a resulttype?](https://github.com/WebAssembly/spec/issues/559)
+### Issues
 
-[proposal multi-value](https://github.com/WebAssembly/multi-value)
+[spec / should functions return a resulttype?](https://github.com/WebAssembly/spec/issues/559)
+[spec / on the use of result type](https://github.com/WebAssembly/spec/issues/1071)
+
+
+### Rationales
+
+#### 1. the abstract syntax is defined to be in 1-to-1 correspondence with the binary representation
+
+that's why `block` and `loop` can only take one "variant-length "
+
+
+### Solution
+
+We are moving to [multi-value](https://github.com/WebAssembly/multi-value) proposal.
+[a better foundation for a mechanization?](https://github.com/WebAssembly/multi-value/issues/23)
+
+> Yes, basing it on the multi-value proposal might be preferable.  -- @rossberg
+
+
 
 
 Structure.v
